@prefix : <http://vsr.informatik.tu-chemnitz.de/projects/2019/growth/wotdl#> .
@prefix owl: <http://www.w3.org/2002/07/owl#> .
@prefix rdf: <http://www.w3.org/1999/02/22-rdf-syntax-ns#> .
@prefix ssn: <http://www.w3.org/ns/ssn/> .
@prefix xml: <http://www.w3.org/XML/1998/namespace> .
@prefix xsd: <http://www.w3.org/2001/XMLSchema#> .
@prefix rdfs: <http://www.w3.org/2000/01/rdf-schema#> .
@prefix owls: <http://www.daml.org/services/owl-s/1.2/Profile.owl#> .
@prefix sosa: <http://www.w3.org/ns/sosa/> .
@base <https://vsr.informatik.tu-chemnitz.de/projects/2019/growth/wotdl> .
@prefix wotdl: <http://vsr.informatik.tu-chemnitz.de/projects/2019/growth/wotdl#> .


<https://vsr.informatik.tu-chemnitz.de/projects/2019/growth/wotdl> rdf:type owl:Ontology ;
                                                                    rdfs:comment "The MQTTWoTDL ontology describes the key concepts of Artificial Intelligence Planning-based End User Development applications for the WoT."^^xsd:string ;
                                                                    owl:versionInfo "1.0" .

#################################################################
#    Annotation properties
#################################################################

###  http://www.semanticweb.org/owl/owlapi/turtle#affects
<http://www.semanticweb.org/owl/owlapi/turtle#affects> rdf:type owl:AnnotationProperty .


###  http://www.semanticweb.org/owl/owlapi/turtle#httpMethod
<http://www.semanticweb.org/owl/owlapi/turtle#httpMethod> rdf:type owl:AnnotationProperty .


#################################################################
#    Object Properties
#################################################################

###  http://vsr.informatik.tu-chemnitz.de/projects/2019/growth/wotdl#affects
wotdl:affects rdf:type owl:ObjectProperty ;
              rdfs:domain wotdl:Effect ;
              rdfs:range wotdl:Parameter ;
              rdfs:comment "The link between an Effect and a Parameter which describes the affects it has on a physical parameter leading to a state change in the environment" ;
              rdfs:label "affects" .


###  http://vsr.informatik.tu-chemnitz.de/projects/2019/growth/wotdl#hasActuation
wotdl:hasActuation rdf:type owl:ObjectProperty ;
                   rdfs:domain wotdl:Transition ;
                   rdfs:range wotdl:Actuation ;
                   rdfs:comment "Relation linking a Transition to the Actuation. " ;
                   rdfs:label "has actuation" .


###  http://vsr.informatik.tu-chemnitz.de/projects/2019/growth/wotdl#hasActuator
wotdl:hasActuator rdf:type owl:ObjectProperty ;
                  rdfs:domain wotdl:CompositeDevice ;
                  rdfs:range wotdl:Actuator ;
                  rdfs:comment "Relation linking a CompositeDevice to the Actuator." ;
                  rdfs:label "has actuator" .


###  http://vsr.informatik.tu-chemnitz.de/projects/2019/growth/wotdl#hasEffect
wotdl:hasEffect rdf:type owl:ObjectProperty ;
                rdfs:domain wotdl:Transition ;
                rdfs:range wotdl:Effect ;
                rdfs:comment "Relation between a Transition and an Effect that describes each transition has an effect on the environment." ;
                rdfs:label "has effect" .


###  http://vsr.informatik.tu-chemnitz.de/projects/2019/growth/wotdl#hasMeasurement
wotdl:hasMeasurement rdf:type owl:ObjectProperty ;
                     rdfs:subPropertyOf owl:topObjectProperty ;
                     rdfs:domain wotdl:Sensor ;
                     rdfs:range wotdl:Measurement ;
                     rdfs:comment "Relation between a Sensor and a Measurement that it is capable of sensing." ;
                     rdfs:label "has measurement" .


###  http://vsr.informatik.tu-chemnitz.de/projects/2019/growth/wotdl#hasParameter
wotdl:hasParameter rdf:type owl:ObjectProperty ;
                   rdfs:domain wotdl:State ;
                   rdfs:range wotdl:Parameter ;
                   rdfs:comment "Describes the relation between a state and a parameter to expresses that each state of the system is described using a set of parameter and values." ;
                   rdfs:label "has parameter" .


###  http://vsr.informatik.tu-chemnitz.de/projects/2019/growth/wotdl#hasPreCondition
wotdl:hasPreCondition rdf:type owl:ObjectProperty ;
                      rdfs:domain wotdl:Transition ;
                      rdfs:range wotdl:PreCondition ;
                      rdfs:comment "Relation from a Transition to a Precondition describing the  transition to next state  under certain Conditions. Used for example to say that in order to turn a lamp off certain conditions apply." ;
                      rdfs:label "has precondition" .


###  http://vsr.informatik.tu-chemnitz.de/projects/2019/growth/wotdl#hasSensor
wotdl:hasSensor rdf:type owl:ObjectProperty ;
                rdfs:domain wotdl:CompositeDevice ;
                rdfs:range wotdl:Sensor ;
                rdfs:comment "Relation linking a CompositeDevice to the Sensor." ;
                rdfs:label "has sensor" .


###  http://vsr.informatik.tu-chemnitz.de/projects/2019/growth/wotdl#hasTransition
wotdl:hasTransition rdf:type owl:ObjectProperty ;
                    rdfs:domain wotdl:Actuator ;
                    rdfs:range wotdl:Transition ;
                    rdfs:comment "Relation from an Actuator to a Transition between the different states of the environment." ;
                    rdfs:label "has transition" .


###  http://vsr.informatik.tu-chemnitz.de/projects/2019/growth/wotdl#measures
wotdl:measures rdf:type owl:ObjectProperty ;
               rdfs:domain wotdl:Measurement ;
               rdfs:range wotdl:Parameter ;
               rdfs:comment "Relation linking a Measurement made by a Sensor to the parameter that was measured. For instance a temperature sensor measures the current temperature." ;
               rdfs:label "measures" .


###  http://vsr.informatik.tu-chemnitz.de/projects/2019/growth/wotdl#on
wotdl:on rdf:type owl:ObjectProperty ;
         rdfs:domain wotdl:PreCondition ;
         rdfs:range wotdl:Parameter ;
         rdfs:comment "Relation from a Transition to an Effect describing the  effects that a certain transition has on the environmental state." ;
         rdfs:label "on" .


###  http://www.semanticweb.org/owl/owlapi/turtle#describesParameter
<http://www.semanticweb.org/owl/owlapi/turtle#describesParameter> rdf:type owl:ObjectProperty ;
                                                                  rdfs:domain <http://www.semanticweb.org/owl/owlapi/turtle#nlpattern> ;
                                                                  rdfs:range wotdl:Parameter ;
                                                                  rdfs:comment "Indicates the parameter on which an effect is described in the natural language pattern"@en ;
                                                                  rdfs:label "describes parameter"@en .


###  http://www.semanticweb.org/owl/owlapi/turtle#direction
<http://www.semanticweb.org/owl/owlapi/turtle#direction> rdf:type owl:ObjectProperty ;
                                                         rdfs:domain <http://www.semanticweb.org/owl/owlapi/turtle#nlpattern> ;
                                                         rdfs:range wotdl:Effect ;
                                                         rdfs:comment "Indicates the direction of the effect on a parameter expressed in a natural language pattern"@en ;
                                                         rdfs:label "direction"@en .


###  http://www.semanticweb.org/owl/owlapi/turtle#locatedIn
<http://www.semanticweb.org/owl/owlapi/turtle#locatedIn> rdf:type owl:ObjectProperty ,
                                                                  owl:TransitiveProperty ;
                                                         rdfs:domain wotdl:Device ,
                                                                     <http://www.semanticweb.org/owl/owlapi/turtle#location> ;
                                                         rdfs:range <http://www.semanticweb.org/owl/owlapi/turtle#location> ;
                                                         rdfs:comment "Relation linking a device or a location to the location it is located in"@en ;
                                                         rdfs:label "located in"@en .


###  http://www.semanticweb.org/owl/owlapi/turtle#scope
<http://www.semanticweb.org/owl/owlapi/turtle#scope> rdf:type owl:ObjectProperty ;
                                                     rdfs:domain wotdl:Effect ;
                                                     rdfs:range wotdl:Device ,
                                                                <http://www.semanticweb.org/owl/owlapi/turtle#location> ;
                                                     rdfs:comment "Defines the scope of the effect, i.e. what is influenced by the defined effect. If not present, then global scope is assumed."@en ;
                                                     rdfs:label "scope"@en .


#################################################################
#    Data properties
#################################################################

###  #operator
<#operator> rdf:type owl:DatatypeProperty ;
            rdfs:domain wotdl:PreCondition ;
            rdfs:range rdfs:Literal .

###  http://vsr.informatik.tu-chemnitz.de/projects/2019/growth/wotdl#decrement
wotdl:decrement rdf:type owl:DatatypeProperty ;
                rdfs:domain wotdl:DecreaseEffect ;
                rdfs:range xsd:decimal ,
                           xsd:double ,
                           xsd:float ;
                rdfs:comment "The amount of decrease an effect has on an environmental parameter" ;
                rdfs:label "Decrement" .


###  http://vsr.informatik.tu-chemnitz.de/projects/2019/growth/wotdl#httpBody
wotdl:httpBody rdf:type owl:DatatypeProperty ;
               rdfs:domain wotdl:HttpRequest ;
               rdfs:range xsd:string ;
               rdfs:comment "OpenAPI 3.0 compliant body specification" ;
               rdfs:label "HTTP body" ;
               rdfs:seeAlso "https://swagger.io/docs/specification/describing-request-body/" .


###  http://vsr.informatik.tu-chemnitz.de/projects/2019/growth/wotdl#httpMethod
wotdl:httpMethod rdf:type owl:DatatypeProperty ;
                 rdfs:domain wotdl:HttpRequest ;
                 rdfs:range xsd:string ;
                 rdfs:comment "HTTP defines a set of request methods to indicate the desired action to be performed for a given resource i.e. get, post, put, delete" ;
                 rdfs:label "HTTP Method" .


###  http://vsr.informatik.tu-chemnitz.de/projects/2019/growth/wotdl#increment
wotdl:increment rdf:type owl:DatatypeProperty ;
                rdfs:domain wotdl:IncreaseEffect ;
                rdfs:range xsd:decimal ,
                           xsd:double ,
                           xsd:float ;
                rdfs:comment "The amount of increase an effect has on an environmental parameter" ;
                rdfs:label "Increment" .


###  http://vsr.informatik.tu-chemnitz.de/projects/2019/growth/wotdl#name
wotdl:name rdf:type owl:DatatypeProperty ;
           rdfs:subPropertyOf owl:topDataProperty ;
           rdfs:domain wotdl:Actuation ,
                       wotdl:CompositeDevice ,
                       wotdl:Device ,
                       wotdl:Parameter ,
                       <http://www.semanticweb.org/owl/owlapi/turtle#location> ;
           rdfs:comment "Describes the name of a physical device, parameter, or actuation" .


###  http://vsr.informatik.tu-chemnitz.de/projects/2019/growth/wotdl#status
wotdl:status rdf:type owl:DatatypeProperty ;
             rdfs:domain wotdl:Effect ,
                         wotdl:PreCondition ;
             rdfs:range xsd:string .


###  http://vsr.informatik.tu-chemnitz.de/projects/2019/growth/wotdl#timeToEffect
wotdl:timeToEffect rdf:type owl:DatatypeProperty ;
                   rdfs:domain wotdl:Effect ;
                   rdfs:range xsd:positiveInteger ;
                   rdfs:comment "The duration it takes for the desired effect to take place" ;
                   rdfs:label "Time To Effect" .


###  http://vsr.informatik.tu-chemnitz.de/projects/2019/growth/wotdl#type
wotdl:type rdf:type owl:DatatypeProperty ;
           rdfs:domain wotdl:CompositeDevice ,
                       wotdl:Parameter ;
           rdfs:range xsd:string .


###  http://vsr.informatik.tu-chemnitz.de/projects/2019/growth/wotdl#url
wotdl:url rdf:type owl:DatatypeProperty ;
          rdfs:domain wotdl:HttpRequest ;
          rdfs:range xsd:string ;
          rdfs:comment "It is a reference to a web resource that specifies its location on a computer network and a mechanism for retrieving it." ;
          rdfs:label "URL" .


###  http://vsr.informatik.tu-chemnitz.de/projects/2019/growth/wotdl#value
wotdl:value rdf:type owl:DatatypeProperty ;
            rdfs:domain wotdl:FixedValueEffect ,
                        wotdl:PreCondition ,
                        wotdl:State ;
            rdfs:range rdfs:Literal ;
            rdfs:comment "It describes the value of a fixed effect type i.e., lamp=on or the value of a precondition lamp=off, or the value of a state. " ;
            rdfs:label "value" .


###  http://vsr.informatik.tu-chemnitz.de/projects/2019/growth/wotdl#waitAfterActuation
wotdl:waitAfterActuation rdf:type owl:DatatypeProperty ;
                         rdfs:domain wotdl:Actuation ;
                         rdfs:range xsd:positiveInteger ;
                         rdfs:comment "The duration it takes before the actuation can take place for example in some cases the device needs to first startup before the actuation can be triggered." ;
                         rdfs:label "Wait After Actuation" .


###  http://vsr.informatik.tu-chemnitz.de/projects/growth/samples/#operator
<http://vsr.informatik.tu-chemnitz.de/projects/growth/samples/#operator> rdf:type owl:DatatypeProperty ;
                                                                         rdfs:domain wotdl:PreCondition ;
                                                                         rdfs:range rdfs:Literal .


###  http://www.semanticweb.org/owl/owlapi/turtle#pattern
<http://www.semanticweb.org/owl/owlapi/turtle#pattern> rdf:type owl:DatatypeProperty ;
                                                       rdfs:domain <http://www.semanticweb.org/owl/owlapi/turtle#nlpattern> ;
                                                       rdfs:range rdfs:Literal ;
                                                       rdfs:comment "The natural language pattern expression, a regular expression"@en ;
                                                       rdfs:label "pattern"@en .


###  https://vsr.informatik.tu-chemnitz.de/projects/2019/growth/wotdl#mqttEndpoint
wotdl:mqttEndpoint rdf:type owl:DatatypeProperty ;
              rdfs:domain wotdl:MqttCommunication ;
              rdfs:range xsd:string ;
              rdfs:comment "Link to the local MQTT broker instance"@en ;
              rdfs:label "mqttEndpoint"@en .


###  https://vsr.informatik.tu-chemnitz.de/projects/2019/growth/wotdl#mqttMessage
wotdl:mqttMessage rdf:type owl:DatatypeProperty ;
             rdfs:domain wotdl:MqttCommunication ;
             rdfs:range xsd:string ;
             rdfs:comment "information that is exchanged"@en ;
             rdfs:label "mqttMessage"@en .


###  https://vsr.informatik.tu-chemnitz.de/projects/2019/growth/wotdl#publishesOn
wotdl:publishesOn rdf:type owl:DatatypeProperty ;
             rdfs:domain wotdl:MqttCommunication ;
             rdfs:range xsd:string ;
             rdfs:comment "MQTT method for sending messages"@en ;
             rdfs:label "publishesOn"@en .


###  https://vsr.informatik.tu-chemnitz.de/projects/2019/growth/wotdl#subscribesTo
wotdl:subscribesTo rdf:type owl:DatatypeProperty ;
              rdfs:domain wotdl:MqttCommunication ;
              rdfs:range xsd:string ;
              rdfs:comment "MQTT message for receiving information"@en ;
              rdfs:label "subscribesTo"@en .


#################################################################
#    Classes
#################################################################

###  http://vsr.informatik.tu-chemnitz.de/projects/2019/growth/wotdl#Actuation
wotdl:Actuation rdf:type owl:Class ;
                rdfs:subClassOf sosa:Actuation ;
                rdfs:comment "An Actuation carries out an (Actuation) Transition to change the state of the world using an Actuator. " ;
                rdfs:label "actuation"@en .


###  http://vsr.informatik.tu-chemnitz.de/projects/2019/growth/wotdl#Actuator
wotdl:Actuator rdf:type owl:Class ;
               rdfs:subClassOf wotdl:Device ;
               rdfs:comment "A device that is used by, or implements, an (Actuation) Procedure that changes the state of the world. " ;
               rdfs:label "actuator"@en .


###  http://vsr.informatik.tu-chemnitz.de/projects/2019/growth/wotdl#CompositeDevice
wotdl:CompositeDevice rdf:type owl:Class ;
                      rdfs:subClassOf wotdl:Device ;
                      rdfs:comment "specifies that a hardware device can have multiple components where each component can be controlled independently. A  CompositeDevice  can have a series of Actuator and Sensor. For example, a Raspberry Pi equipped with a SenseHat is a  CompositeDevice with a set of sensors and actuators i.e., LED board that are connected to it. " ;
                      rdfs:label "composite device"@en .


###  http://vsr.informatik.tu-chemnitz.de/projects/2019/growth/wotdl#DecreaseEffect
wotdl:DecreaseEffect rdf:type owl:Class ;
                     rdfs:subClassOf wotdl:Effect ;
                     rdfs:comment "It is used for decreasing a parameter" ;
                     rdfs:label "decrease effect"@en .


###  http://vsr.informatik.tu-chemnitz.de/projects/2019/growth/wotdl#Device
wotdl:Device rdf:type owl:Class ;
             rdfs:comment "A device that is used by, or implements, an (Actuation) Procedure that changes the state of the world" ;
             rdfs:label "device"@en .


###  http://vsr.informatik.tu-chemnitz.de/projects/2019/growth/wotdl#Effect
wotdl:Effect rdf:type owl:Class ;
             rdfs:comment "The transformation of Actuations performed by Actuators and the affects it has on a physical parameter leading to a state change in the environment" ;
             rdfs:label "effect"@en .


###  http://vsr.informatik.tu-chemnitz.de/projects/2019/growth/wotdl#FixedValueEffect
wotdl:FixedValueEffect rdf:type owl:Class ;
                       rdfs:subClassOf wotdl:Effect ;
                       rdfs:comment "It is used for assigning constant values to a parameter" ;
                       rdfs:label "fixed value effect"@en .


###  http://vsr.informatik.tu-chemnitz.de/projects/2019/growth/wotdl#GoalState
wotdl:GoalState rdf:type owl:Class ;
                rdfs:subClassOf wotdl:State ;
                rdfs:comment "It refers to the desired state of the environment" ;
                rdfs:label "goal state"@en .


###  http://vsr.informatik.tu-chemnitz.de/projects/2019/growth/wotdl#HttpRequest
wotdl:HttpRequest rdf:type owl:Class ;
                  rdfs:subClassOf wotdl:Actuation ,
                                  wotdl:Measurement ;
                  rdfs:comment "Provides all the required information to execute an HTTP request to perform either Actuation or Measurement. The HTTPRequest includes HTTPMethod (GET, POST, PUT), HTTPheader, URL, and the body." ;
                  rdfs:label "HTTP request"@en .


###  http://vsr.informatik.tu-chemnitz.de/projects/2019/growth/wotdl#IncreaseEffect
wotdl:IncreaseEffect rdf:type owl:Class ;
                     rdfs:subClassOf wotdl:Effect ;
                     rdfs:comment "for increasing a parameter" ;
                     rdfs:label "increase effect"@en .


###  http://vsr.informatik.tu-chemnitz.de/projects/2019/growth/wotdl#InitialState
wotdl:InitialState rdf:type owl:Class ;
                   rdfs:subClassOf wotdl:State ;
                   rdfs:comment "It refers to the state at the start of planning." ;
                   rdfs:label "initial state"@en .


###  http://vsr.informatik.tu-chemnitz.de/projects/2019/growth/wotdl#Measurement
wotdl:Measurement rdf:type owl:Class ;
                  rdfs:comment "It is triggered on a Sensor device to measure the value of a Parameter." ;
                  rdfs:label "measurement"@en .


###  http://vsr.informatik.tu-chemnitz.de/projects/2019/growth/wotdl#Parameter
wotdl:Parameter rdf:type owl:Class ;
                rdfs:comment "expresses the facts known about each State." ;
                rdfs:label "parameter"@en .


###  http://vsr.informatik.tu-chemnitz.de/projects/2019/growth/wotdl#PreCondition
wotdl:PreCondition rdf:type owl:Class ;
                   rdfs:comment "In order for a Transition to be applied  to reach the next state, itâ€™s Precondition must hold true. " ;
                   rdfs:label "precondition"@en .


###  http://vsr.informatik.tu-chemnitz.de/projects/2019/growth/wotdl#Sensor
wotdl:Sensor rdf:type owl:Class ;
             rdfs:subClassOf wotdl:Device ,
                             ssn:Sensor ;
             rdfs:comment "Device, agent, or software (simulation) involved in, or implementing, a Procedure. Sensors respond to a Stimulus, e.g., a change in the environment, or Input data composed from the Results of prior Measurement, and generate a Result. Sensors are subclass of Device. Example temperature sensor, air quality sensor, humidity sensor, motion sensor etc." ,
                          "Sensors are a subclass of Device which measures the current state of the environment. Examples include temperature sensor, humidity sensor, motion sensor. " ;
             rdfs:label "sensor"@en .


###  http://vsr.informatik.tu-chemnitz.de/projects/2019/growth/wotdl#State
wotdl:State rdf:type owl:Class ;
            rdfs:comment "It is used to describe the state of the physical environment" ;
            rdfs:label "state"@en .


###  http://vsr.informatik.tu-chemnitz.de/projects/2019/growth/wotdl#ToggleEffect
wotdl:ToggleEffect rdf:type owl:Class ;
                   rdfs:subClassOf wotdl:Effect ;
                   rdfs:comment "for switching between the possible values of parameter" ;
                   rdfs:label "toggle effect"@en .


###  http://vsr.informatik.tu-chemnitz.de/projects/2019/growth/wotdl#Transition
wotdl:Transition rdf:type owl:Class ;
                 rdfs:comment "describes the Effect i.e., that is the dynamic change between different states of the environment which are intended to be caused by the Actuation-the expected behavior which may not necessarily occur due to external influences, unpredicted behavior, etc. performed by Actuators and Precondition." ;
                 rdfs:label "transition"@en .


###  http://www.semanticweb.org/owl/owlapi/turtle#location
<http://www.semanticweb.org/owl/owlapi/turtle#location> rdf:type owl:Class ;
                                                        rdfs:comment "The location in which a device is located. Also used to expresses structure of nested locations, i.e. locations located in other locations."@en ;
                                                        rdfs:label "location"@en .


###  http://www.semanticweb.org/owl/owlapi/turtle#nlpattern
<http://www.semanticweb.org/owl/owlapi/turtle#nlpattern> rdf:type owl:Class ;
                                                         rdfs:comment "A natural language pattern describing the relationship between an expression in natural language, the parameter which is effected and the direction of the effect."@en ;
                                                         rdfs:label "natural language pattern"@en .


###  http://www.w3.org/ns/sosa/Actuation
sosa:Actuation rdf:type owl:Class .


###  http://www.w3.org/ns/ssn/Sensor
ssn:Sensor rdf:type owl:Class .


###  https://vsr.informatik.tu-chemnitz.de/projects/2019/growth/wotdl#MqttCommunication
wotdl:MqttCommunication rdf:type owl:Class ;
                   rdfs:subClassOf wotdl:Actuation ,
                                   wotdl:Measurement ;
                   rdfs:comment "Provides all the required information to execute an MQTT request to perform either Actuation or Measurement. The MQTT Request contains mqttMessage, mqttEndpoint, subscribesTo and publishesOn." ;
                   rdfs:label "MqttCommunication"@en .


#################################################################
#    Individuals
#################################################################


<#Fan>
    a wotdl:Actuator ;
    wotdl:hasTransition <#TurnOffTransition>, <#FanSpeedSetTransition> , <#IncreaseSpeedTransition>, <#DecreaseSpeedTransition>;
    wotdl:name "dc_motor_fan"^^xsd:string ;
    wotdl:type "fan".


<#TurnOffTransition>
	a wotdl:Transition;
	wotdl:hasPreCondition <#FanPC>;
	wotdl:hasActuation <#FanTurnOff> ;
  wotdl:hasEffect <#IncreaseTemperature> , <#FanPowerState> .


<#FanPC>
	a wotdl:PreCondition;
	wotdl:on <#FanPowerState>;
	wotdl:operation "op:numeric-equal";
	wotdl:value "on"^^xsd:string .

<#FanPowerState>
    a wotdl:Parameter ;
    wotdl:name "FanPowerState";
    wotdl:type "OnOff".


 <#FanTurnOff>
  	a wotdl:HttpRequest, wotdl:MqttCommunication, wotdl:Actuation;
  	wotdl:httpMethod "POST"^^xsd:string;
	wotdl:name "fan_turn_off"^^xsd:string;
	wotdl:url "http://10.0.1.200/fan/off"^^xsd:string ;
    wotdl:mqttEndpoint "mqtt://localhost"^^xsd:string ;
    wotdl:mqttMessage """contentType: application/json
payload:
    type: string"""^^xsd:string ;
    wotdl:subscribesTo "fan/3/off"^^xsd:string .


<#IncreaseTemperature>
  a wotdl:IncreaseEffect ;
  wotdl:affects <#Temperature> .


<#Temperature>
    a wotdl:Parameter ;
    wotdl:name "Temperature";
    wotdl:type xsd:decimal .


<#FanSpeedSetTransition>
	a wotdl:Transition;
	wotdl:hasActuation <#FanSet> ;
    wotdl:hasEffect <#FanOnEffect> , <#FanSetEffect> .


<#FanSet>
    a wotdl:HttpRequest, wotdl:MqttCommunication, wotdl:Actuation ;
    wotdl:httpBody """required: true
content:
  application/x-www-form-urlencoded:
    schema:
      type: object
      properties:
        target_speed:
          type: number
      required:
        - target_speed"""^^xsd:decimal ;
    wotdl:httpMethod "POST"^^xsd:string ;
    wotdl:name "fan_set"^^xsd:string ;
    wotdl:url "http://10.0.1.200/fan"^^xsd:string ;
    wotdl:mqttEndpoint "mqtt://localhost"^^xsd:string ;
    wotdl:mqttMessage """contentType: application/json
payload:
    type: string"""^^xsd:string ;
    wotdl:subscribesTo "fan/3/setFanSpeed"^^xsd:string .


<#FanOnEffect>
    a wotdl:FixedValueEffect ;
    wotdl:affects <#FanPowerState> ;
    wotdl:value "on"^^xsd:string .


<#FanSetEffect>
   a wotdl:FixedValueEffect ;
   wotdl:affects <#Speed> , <#Temperature> .


<#Speed>
    a wotdl:Parameter ;
    wotdl:name "Speed";
    wotdl:type xsd:decimal .

<#IncreaseSpeedTransition>
	a wotdl:Transition;
	wotdl:hasPreCondition <#FanPC>;
	wotdl:hasActuation <#IncreaseFanSpeed>;
	wotdl:hasEffect <#DecreaseTemperature> , <#IncreaseSpeed>.



<#IncreaseFanSpeed>
    a wotdl:HttpRequest, wotdl:MqttCommunication, wotdl:Actuation ;
    wotdl:httpBody """required: true
content:
  application/x-www-form-urlencoded:
    schema:
      type: object
      properties:
        increment:
          type: number
      required:
        - increment"""^^xsd:decimal ;
    wotdl:httpMethod "POST"^^xsd:string ;
    wotdl:name "increase_fan_speed"^^xsd:string ;
    wotdl:url "http://10.0.1.200/fan/increase"^^xsd:string ;
    wotdl:mqttEndpoint "mqtt://localhost"^^xsd:string ;
    wotdl:mqttMessage """contentType: application/json
payload:
    type: string"""^^xsd:string ;
                  wotdl:subscribesTo "fan/3/increaseSpeed"^^xsd:string .


<#DecreaseTemperature>
  a wotdl:DecreaseEffect ;
  wotdl:affects <#Temperature> .


<#IncreaseSpeed>
  a wotdl:IncreaseEffect ;
  wotdl:affects <#Speed> ;
  wotdl:increment "1"^^xsd:decimal .


<#DecreaseSpeedTransition>
	a wotdl:Transition;
	wotdl:hasPreCondition <#FanPC>;
	wotdl:hasActuation <#DecreaseFanSpeed>;
	wotdl:hasEffect <#IncreaseTemperature> , <#DecreaseSpeed>.



<#DecreaseFanSpeed>
    a wotdl:HttpRequest, wotdl:MqttCommunication, wotdl:Actuation ;
    wotdl:httpBody """required: true
content:
  application/x-www-form-urlencoded:
    schema:
      type: object
      properties:
        decrement:
          type: number
      required:
        - decrement"""^^xsd:decimal ;
    wotdl:httpMethod "POST"^^xsd:string ;
    wotdl:name "decrease_fan_speed"^^xsd:string ;
    wotdl:url "http://10.0.1.200/fan/decrease"^^xsd:string ;
    wotdl:mqttEndpoint "mqtt://localhost"^^xsd:string ;
    wotdl:mqttMessage """contentType: application/json
payload:
    type: string"""^^xsd:string ;
    wotdl:subscribesTo "fan/3/decreaseSpeed"^^xsd:string .



<#DecreaseSpeed>
  a wotdl:IncreaseEffect ;
  wotdl:affects <#Speed> ;
  wotdl:decrement "1"^^xsd:decimal .


<#light>
    a wotdl:Sensor ;
    wotdl:hasMeasurement <#LightM>;
    wotdl:name "light_sensor"^^xsd:string ;
    wotdl:type "fan".


<#LightM>
    a wotdl:HttpRequest, wotdl:MqttCommunication, wotdl:Measurement ;
    wotdl:measures <#AmbientLuminosity> ;
    wotdl:httpMethod "GET"^^xsd:string ;
    wotdl:name "get_light_intensity"^^xsd:string ;
    wotdl:url "http://10.0.1.200/ambientlight"^^xsd:string ;
    wotdl:mqttEndpoint "mqtt://localhost"^^xsd:string ;
    wotdl:mqttMessage """contentType: application/json
payload:
    type: object
      properties:
        id:
          type: integer
          minimum: -10
          description: Id of the light sensor
        light:
          type: integer
          minimum: 0
          description: Light measured as lumen.
        sentAt:
          type: string
          format: date-time
          description: Date and time when the message was sent."""^^xsd:string ;
    wotdl:publishesOn "light"^^xsd:string .

<#AmbientLuminosity>
  a wotdl:Parameter;
  wotdl:name "AmbientLuminosity".

  <#PhilipsHue>
    a wotdl:CompositeDevice ;
    wotdl:hasActuator <#LampActuator> ;
    wotdl:name "philipshue"^^xsd:string ;
    wotdl:type "lamp"^^xsd:string .


<#LampActuator>
    a wotdl:Actuator ;
    wotdl:name "philipshue"^^xsd:string ;
    wotdl:hasTransition <#LampOffTransition> , <#LampOnTransition>.

<#LampOffTransition>
    a wotdl:Transition ;
    wotdl:hasPreCondition <#LampOffPrecondition>;
    wotdl:hasActuation <#LampOff> ;
    wotdl:hasEffect <#DecreaseBrightness> , <#TurnLampOff> .


<#LampOffPrecondition>
    a wotdl:PreCondition ;
    wotdl:on <#LampPowerState> ;
    wotdl:value "on"^^rdfs:Literal .

<#LampOff>
    a wotdl:MqttCommunication, wotdl:HttpRequest, wotdl:Actuation ;
    wotdl:httpMethod "PUT"^^xsd:string ;
    wotdl:url "http://10.0.1.200/lights/off"^^xsd:string ;
    wotdl:name "switch_off_lamp"^^xsd:string ;
    wotdl:subscribesTo "light/1/off"^^xsd:string ;
    wotdl:mqttEndpoint "mqtt://localhost"^^xsd:string ;
    wotdl:mqttMessage """contentType: application/json
        payload:"""^^xsd:string .



<#DecreaseBrightness>
    a wotdl:DecreaseEffect ;
    :affects :AmbientLuminosity .

<#AmbientLuminosity>
    a wotdl:Parameter;
    wotdl:name "AmbientLuminosity".


<#TurnLampOff>
    a wotdl:FixedValueEffect ;
    wotdl:affects :LampPowerState ;
    wotdl:value "off"^^rdfs:Literal .

<#LampOnTransition>
    a wotdl:Transition ;
    wotdl:hasPreCondition <#LampOnPrecondition> ;
    wotdl:hasActuation <#LampOn> ;
    wotdl:hasEffect <#IncreaseBrightness> , <#TurnLampOn> .

<#LampOnPrecondition>
    a wotdl:PreCondition ;
    wotdl:on <#LampPowerState> ;
    wotdl:value "off"^^rdfs:Literal .

<#LampPowerState>
    a wotdl:Parameter ;
    wotdl:name "LampPowerState"^^xsd:string ;
    wotdl:type "onoff".


<#LampOn>
    a wotdl:HttpRequest, wotdl:MqttCommunication, wotdl:Actuation ;
    wotdl:subscribesTo "light/1/on" ;
    wotdl:mqttEndpoint "mqtt://localhost" ;
    wotdl:mqttMessage """contentType: application/json
        payload:"""^^xsd:string ;
    wotdl:httpMethod "PUT"^^xsd:string ;
    wotdl:name "switch_on_lamp"^^xsd:string ;
    wotdl:url "http://10.0.1.200/lights/on"^^xsd:string .


<#TurnLampOn> rdf:type wotdl:FixedValueEffect ;
             wotdl:affects <#LampPowerState> ;
             wotdl:value "on"^^rdfs:Literal .


<#temperature>
    a wotdl:Sensor ;
    wotdl:hasMeasurement <#TemperatureM>;
  wotdl:name "temperature_humidity_sensor"^^xsd:string ;
    wotdl:type "temperature".

<#TemperatureM>
    a wotdl:HttpRequest, wotdl:MqttCommunication, wotdl:Measurement ;
    wotdl:measures <#AmbientTemperature> ;
    wotdl:httpMethod "GET"^^xsd:string ;
    wotdl:name "get_temperature"^^xsd:string ;
    wotdl:url "http://10.0.1.200/temperature"^^xsd:string ;
    wotdl:mqttEndpoint "mqtt://localhost"^^xsd:string ;
    wotdl:mqttMessage """contentType: application/json
payload:
    type: object
      properties:
        id:
          type: integer
          minimum: -10
          description: Id of the temperature sensor
        temperature:
          type: integer
          minimum: 0
          description: Temperature measured as celcuis.
        sentAt:
          type: string
          format: date-time
          description: Date and time when the message was sent."""^^xsd:string ;
              wotdl:publishesOn "temperature"^^xsd:string .

<#AmbientTemperature>
  a wotdl:Parameter;
  wotdl:name "AmbientTemperature".

<#humidity>
    a wotdl:Sensor ;
    wotdl:hasMeasurement <#HumidityM>;
  wotdl:name "temperature_humidity_sensor"^^xsd:string ;
    wotdl:type "humidity".

<#HumidityM>
    a wotdl:HttpRequest, wotdl:MqttCommunication, wotdl:Measurement ;
    wotdl:measures <#AmbientHumidity> ;
    wotdl:httpMethod "GET"^^xsd:string ;
    wotdl:name "get_humidity"^^xsd:string ;
    wotdl:url "http://10.0.1.200/humidity"^^xsd:string ;
    wotdl:mqttEndpoint "mqtt://localhost"^^xsd:string ;
    wotdl:mqttMessage """contentType: application/json
payload:
    type: object
      properties:
        id:
          type: integer
          minimum: -10
          description: Id of the humidity sensor
        humidity:
          type: integer
          minimum: 0
          description: Humidity measured as percentage.
        sentAt:
          type: string
          format: date-time
          description: Date and time when the message was sent."""^^xsd:string ;
           wotdl:publishesOn "humidity"^^xsd:string .

<#AmbientHumidity>
  a wotdl:Parameter;
  wotdl:name "AmbientHumidity".



<#Thermostat>
    a wotdl:Actuator ;
    wotdl:hasTransition :ThermostatTransition ;
    wotdl:name "thermostat"^^xsd:string ;
    wotdl:type "thermostat".


<#ThermostatTransition>
    a wotdl:Transition ;
    wotdl:hasActuation <#ThermostatSet> ;
    wotdl:hasEffect <#HeatingOnEffect> , <#ThermostatEffect> .


<#ThermostatSet>
  a wotdl:HttpRequest, wotdl:MqttCommunication, wotdl:Actuation ;
  wotdl:httpBody """required: true
content:
  application/x-www-form-urlencoded:
    schema:
      type: object
      properties:
        targetTemperature:
          type: number
      required:
        - targetTemperature"""^^xsd:string ;
  wotdl:httpMethod "PUT"^^xsd:string ;
  wotdl:name "thermostat_set"^^xsd:string ;
  wotdl:url "http://10.0.1.200/thermostat"^^xsd:string ;
  wotdl:mqttEndpoint "mqtt://localhost"^^xsd:string ;
  wotdl:mqttMessage """contentType: application/json
payload:
    type: string"""^^xsd:string ;
  wotdl:subscribesTo "thermostat/5/setTemperature"^^xsd:string .

<#HeatingOnEffect>
    a wotdl:FixedValueEffect ;
    wotdl:affects <#HeatingPowerState> ;
    wotdl:value "on"^^xsd:string .


  <#ThermostatEffect>
    a wotdl:IncreaseEffect ;
    wotdl:affects <#Temperature> .


<#Temperature>
    a wotdl:Parameter ;
    wotdl:name "Temperature";
    wotdl:type xsd:decimal .


<#HeatingPowerState>
    a wotdl:Parameter ;
    wotdl:name "HeatingPowerState";
    wotdl:type "OnOff".


<#Heating>
  a wotdl:Actuator ;
  wotdl:hasTransition <#HeatingOffTransition>, <#HeatingOnTransition>;
  wotdl:name "relay_heating"^^xsd:string ;
  wotdl:type "heating".


<#HeatingOffTransition>
  a wotdl:Transition;
  wotdl:hasPreCondition <#HeatingOffPrecondition>;
  wotdl:hasActuation <#HeatingOff>;
  wotdl:hasEffect <#DecreaseTemperature>, <#HeatingOffEffect>.

<#HeatingOffPrecondition>
  a wotdl:PreCondition ;
  wotdl:on <#HeatingPowerState> ;
  wotdl:value "on"^^xsd:string .


<#HeatingOff>
  a wotdl:HttpRequest, wotdl:MqttCommunication, wotdl:Actuation ;
  wotdl:httpMethod "POST"^^xsd:string ;
  wotdl:name "deactivate_heating"^^xsd:string ;
  wotdl:url "http://10.0.1.200/heating/off"^^xsd:string ;
  wotdl:mqttEndpoint "mqtt://localhost"^^xsd:string ;
  wotdl:mqttMessage """contentType: application/json
payload:
    type: string"""^^xsd:string ;
  wotdl:subscribesTo "heating/2/off"^^xsd:string .


<#DecreaseTemperature>
  a wotdl:DecreaseEffect ;
  wotdl:affects <#Temperature> .


<#HeatingOffEffect>
  a wotdl:FixedValueEffect ;
  wotdl:affects <#HeatingPowerState> ;
  wotdl:value "off"^^xsd:string .


<#HeatingOnTransition>
  a wotdl:Transition ;
  wotdl:hasActuation <#HeatingOn> ;
  wotdl:hasEffect <#HeatingOnEffect> , <#IncreaseTemperature> ;
  wotdl:hasPreCondition <#HeatingOnPrecondition> .


<#HeatingOn>
  a wotdl:HttpRequest, wotdl:MqttCommunication, wotdl:Actuation ;
  wotdl:httpBody """required: true
content:
  application/x-www-form-urlencoded:
    schema:
      type: object
      properties:
        power:
          type: number
      required:
        - power"""^^xsd:string ;
  wotdl:httpMethod "POST"^^xsd:string ;
  wotdl:name "activate_heating"^^xsd:string ;
  wotdl:url "http://10.0.1.200/heating/on"^^xsd:string ;
  wotdl:mqttEndpoint "mqtt://localhost"^^xsd:string ;
  wotdl:mqttMessage """contentType: application/json
payload:
    type: string"""^^xsd:string ;
  wotdl:subscribesTo "heating/2/on"^^xsd:string .


<#HeatingOnEffect>
  a wotdl:FixedValueEffect ;
  wotdl:affects <#HeatingPowerState> ;
  wotdl:value "on"^^xsd:string .


<#IncreaseTemperature>
  a wotdl:IncreaseEffect ;
  wotdl:affects <#Temperature> .


<#HeatingOnPrecondition>
  a wotdl:PreCondition ;
  wotdl:on <#HeatingPowerState> ;
  wotdl:value "off"^^xsd:string .


<#samsungtv>
    a wotdl:Actuator, wotdl:Device ;
    wotdl:hasTransition <#tvOnTransition>;
    wotdl:hasTransition <#tvOffTransition>;
    wotdl:name "samsung_tv"^^xsd:string ;
    wotdl:type "tv"^^xsd:string .



<#tvOnTransition>
    a wotdl:Transition ;
    wotdl:hasActuation <#TvOn> .


<#tvOffTransition>
    a wotdl:Transition ;
    wotdl:hasActuation <#TvOff> .


<#TvOn>
    a wotdl:HttpRequest, wotdl:MqttCommunication, wotdl:Actuation;
    wotdl:httpMethod "POST"^^xsd:string ;
    wotdl:name "switch_on_tv"^^xsd:string ;
    wotdl:url "http://10.0.1.200/tv/{path-param}/needed/on"^^xsd:string ;
    wotdl:httpBody """required: true
content:
  application/x-www-form-urlencoded:
    schema:
      type: object
      properties:
        power:
          type: number
      required:
        - power"""^^xsd:string ;
    wotdl:mqttEndpoint "mqtt://localhost"^^xsd:string ;
    wotdl:mqttMessage """contentType: application/json
payload:
    type: string"""^^xsd:string ;
    wotdl:subscribesTo "tv/4/on"^^xsd:string .

<#TvOff>
    a wotdl:HttpRequest, wotdl:MqttCommunication, wotdl:Actuation;
    wotdl:httpMethod "GET"^^xsd:string ;
    wotdl:name "switch_off_tv"^^xsd:string ;
    wotdl:url "http://10.0.1.200/tv/{path-param}/needed/off?queryParam1={myQueryStuff}"^^xsd:string ;
    wotdl:mqttEndpoint "mqtt://localhost"^^xsd:string ;
    wotdl:mqttMessage """contentType: application/json
payload:
    type: string"""^^xsd:string ;
    wotdl:subscribesTo "tv/4/off"^^xsd:string .